theories/SpecNotations.v
@@ -10,7 +10,6 @@ Bind Scope list_scope with stores.
 Infix "*" := t_prod.
 
 Notation "G ⊢ v 'in' t" := (Jv G v t) (at level 90).
-Notation "p ⊢ v ⇓ N" := (bigv p v N) (at level 90).
 
 Infix "|-" := P_with (at level 30).
 
